add printers and test of fa2token

execution/tests/FA2TokenTests.v
@@ -1,13 +1,14 @@
+
+
+
+
+Module FA2ClientContract.
 From ConCert Require Import Blockchain LocalBlockchain FA2Token FA2Interface.
 From ConCert Require Import Serializable.
 From ConCert Require Import LocalBlockchainTests.
 From ConCert Require Import BoundedN.
 Require Import Extras.
 
-
-
-
-Module FA2CallerContract.
 From Coq Require Import Morphisms.
 Require Import Monads.
 Require Import Extras.
@@ -17,25 +18,26 @@ From RecordUpdate Require Import RecordUpdate.
 From Coq Require Import List.
 Require Import Serializable.
 Require Import Blockchain.
+Require Import ZArith.
 Import ListNotations.
 Import RecordSetNotations.
 
-Section FA2Caller.
+Section FA2Client.
 Context {BaseTypes : ChainBase}.
 (* Context {FA2ContractAddr : Address}. *)
 Set Primitive Projections.
 Set Nonrecursive Elimination Schemes.
-(* Open Scope N_scope. *)
+Open Scope N_scope.
 
-Inductive Msg' :=
-  | Call_fa2_is_operator : is_operator_param -> Msg'
-. 
+Inductive FA2ClientMsg :=
+  | Call_fa2_is_operator : is_operator_param -> FA2ClientMsg. 
 
-Definition FA2CallerMsg : Type := is_operator_response + Msg'.
+Definition Msg := @FA2ReceiverMsg BaseTypes FA2ClientMsg.
 
 Record State := 
   build_state {
-  fa2_caddr : Address
+  fa2_caddr : Address;
+  bit : N;
 }.
 
 Record Setup := 
@@ -44,20 +46,28 @@ Record Setup :=
 }.
 
 Instance state_settable : Settable _ :=
-  settable! build_state <fa2_caddr>.
+  settable! build_state <fa2_caddr; bit>.
 Instance setup_settable : Settable _ :=
   settable! build_setup <fa2_caddr_>.
 
 Section Serialization.
+Global Instance FA2ClientMsg_serializable : Serializable FA2ClientMsg :=
+  Derive Serializable FA2ClientMsg_rect <Call_fa2_is_operator>.
 
 Global Instance setup_serializable : Serializable Setup :=
   Derive Serializable Setup_rect <build_setup>.
 
-Global Instance msg'_serializable : Serializable Msg' :=
-  Derive Serializable Msg'_rect <Call_fa2_is_operator>.
+Global Instance Msg_serializable' : Serializable (@FA2ReceiverMsg BaseTypes FA2ClientMsg) :=
+Derive Serializable (@FA2ReceiverMsg_rect BaseTypes FA2ClientMsg) <
+  (@receive_balance_of_param BaseTypes FA2ClientMsg), 
+  (@receive_total_supply_param BaseTypes FA2ClientMsg), 
+  (@receive_metadata_callback BaseTypes FA2ClientMsg), 
+  (@receive_is_operator BaseTypes FA2ClientMsg), 
+  (@transfer_hook  BaseTypes FA2ClientMsg), 
+  (@other_msg BaseTypes FA2ClientMsg)>.
 
-About FA2CallerMsg.
-Import Serializable.
+Global Instance Msg_serializable : Serializable FA2Client.Msg := Msg_serializable'.
+(* Import Serializable.
 Ltac make_serializable eliminator ctors :=
   let ser := make_serializer eliminator in
   let elim_ty := type of eliminator in
@@ -74,39 +84,130 @@ Global Program Instance msg_serializable : Serializable FA2CallerMsg :=
 |}.
 Next Obligation.
 intros. rewrite deserialize_serialize_sum. 
-reflexivity. Qed.
+reflexivity. Qed. *)
 
 Global Instance state_serializable : Serializable State :=
 	Derive Serializable State_rect <build_state>.
 
 End Serialization.
   
+Definition init (chain : Chain)
+								(ctx : ContractCallContext)
+								(setup : Setup) : option State := 
+  Some {|
+    fa2_caddr := setup.(fa2_caddr_);
+    bit := 0;
+	|}.
 
-End FA2Caller.
-End FA2CallerContract.
+Definition receive (chain : Chain)
+						 			 (ctx : ContractCallContext)
+									 (state : State)
+									 (maybe_msg : option FA2Client.Msg)
+									 : option (State * list ActionBody) :=
+	match maybe_msg with
+  | Some (receive_is_operator is_op_response) => Some (state<| bit:= 1|>, [])
+  | Some (other_msg (Call_fa2_is_operator is_op_param)) => Some (state<| bit := 2|>, [])
+  | _ => None 
+	end.
 
+Ltac solve_contract_proper :=
+  repeat
+    match goal with
+    | [|- ?x _  = ?x _] => unfold x
+    | [|- ?x _ _ = ?x _ _] => unfold x
+    | [|- ?x _ _ _ = ?x _ _ _] => unfold x
+    | [|- ?x _ _ _ _ = ?x _ _ _ _] => unfold x
+    | [|- ?x _ _ _ _ = ?x _ _ _ _] => unfold x
+    | [|- ?x _ _ _ _ _ = ?x _ _ _ _ _] => unfold x
+    | [|- Some _ = Some _] => f_equal
+    | [|- pair _ _ = pair _ _] => f_equal
+    | [|- (if ?x then _ else _) = (if ?x then _ else _)] => destruct x
+    | [|- match ?x with | _ => _ end = match ?x with | _ => _ end ] => destruct x
+    | [H: ChainEquiv _ _ |- _] => rewrite H in *
+    | _ => subst; auto
+    end.
 
+Lemma init_proper :
+  Proper (ChainEquiv ==> eq ==> eq ==> eq) FA2Client.init.
+Proof. repeat intro; solve_contract_proper.	Qed.
 
-From ConCert.Execution.QCTests Require Import 
-  ChainGens TestUtils ChainPrinters SerializablePrinters TraceGens.
+Lemma receive_proper :
+  Proper (ChainEquiv ==> eq ==> eq ==> eq ==> eq) FA2Client.receive.
+Proof. repeat intro; solve_contract_proper. Qed.
 
+Definition contract : Contract Setup Msg State :=
+  build_contract FA2Client.init init_proper FA2Client.receive receive_proper.
+
+End FA2Client.
+
+End FA2ClientContract.
+
+Global Set Warnings "-extraction-logical-axiom".
 Require Import ZArith Strings.String.
-
 From QuickChick Require Import QuickChick. Import QcNotation.
 From ExtLib.Structures Require Import Functor Applicative.
-From ExtLib.Structures Require Import Monads.
-Import MonadNotation. Open Scope monad_scope.
-From Coq Require Import List. Import ListNotations.
-From Coq Require Import Morphisms.
-From Coq Require Import Program.Basics.
-Require Import Containers.
 
+From ConCert Require Import Blockchain.
+From ConCert Require Import LocalBlockchain.
+From ConCert Require Import Serializable.
+From ConCert Require Import BoundedN.
+From ConCert Require Import LocalBlockchainTests.
+From ConCert Require Import Containers.
+From ConCert Require Import FA2Token FA2Interface.
+From RecordUpdate Require Import RecordUpdate.
+Import RecordSetNotations.
+
+Require Import Extras.
+
+From ConCert.Execution.QCTests Require Import 
+	ChainGens TestUtils ChainPrinters SerializablePrinters TraceGens FA2Printers.
+(* For monad notations *)
+(* From ExtLib.Structures Require Import Monads.
+Import MonadNotation. Open Scope monad_scope. *)
+From Coq Require Import List Int.
+Import BoundedN.Stdpp.
 Import LocalBlockchain.
 Import ListNotations.
+Close Scope address_scope.
 
-Notation "f 'o' g" := (compose f g) (at level 50).
+Section Printers.
+Local Open Scope string_scope.
 
-Definition LocalChainBase : ChainBase := ChainGens.LocalChainBase.
+Instance showFA2ClientMsg : Show FA2ClientContract.FA2ClientMsg :=
+{|
+	show m := match m with
+						| FA2ClientContract.Call_fa2_is_operator param => "call_fa2_is_operator " ++ show param 
+						end
+|}.
+
+Instance showFA2ClientContractMsg : Show FA2ClientContract.Msg :=
+{|
+	show m := show m
+|}.
+
+Instance showFA2ClientState : Show FA2ClientContract.State :=
+{|
+  show t := "FA2ClientContractState{" 
+            ++ "fa2_caddr: " ++ show t.(FA2ClientContract.fa2_caddr) ++ sep 
+            ++ "bit: " ++ show t.(FA2ClientContract.bit) 
+            ++ "}"
+|}.
+
+Instance showFA2Setup : Show FA2ClientContract.Setup :=
+{|
+  show t := "FA2ClientContractSetup{" 
+            ++ "fa2_caddr_: " ++ show t.(FA2ClientContract.fa2_caddr_) 
+            ++ "}"
+|}.
+       
+Close Scope string_scope.
+End Printers.
+
+(* Notation "f 'o' g" := (compose f g) (at level 50). *)
+
+(* Definition LocalChainBase : ChainBase := ChainGens.LocalChainBase. *)
+(* Let BaseTypes := ChainGens.LocalChainBase. *)
+(* Instance BaseTypes : ChainBase := ChainGens.LocalChainBase. *)
 (** example policies *)
 
 (* the policy which allows only token owners to transfer their own tokens. *)
@@ -127,20 +228,68 @@ Definition own_policy1 : permissions_descriptor := {|
   descr_custom := None;
 |}.
 
-
 Definition token_setup := FA2Token.build_setup [] own_policy .
-Definition deploy_fa2token := create_deployment 0 FA2Token.contract token_setup.
+Definition deploy_fa2token : @ActionBody Base := create_deployment 0 FA2Token.contract token_setup.
 
-Let contract_base_addr := BoundedN.of_Z_const AddrSize 128%Z.
+Definition token_contract_base_addr : Address := BoundedN.of_Z_const AddrSize 128%Z.
 
-Definition chain_with_token_deployed :=  
+Definition token_client_setup := FA2ClientContract.build_setup token_contract_base_addr.
+Definition deploy_fa2token_client : @ActionBody Base := create_deployment 0 FA2ClientContract.contract token_client_setup.
+Definition client_contract_addr : Address := BoundedN.of_Z_const AddrSize 129%Z.
+
+
+Definition chain_with_token_deployed : LocalChain :=  
   unpack_option (my_add_block lc_initial 
   [
     build_act creator (act_transfer person_1 10);
     build_act creator (act_transfer person_2 10);
     build_act creator (act_transfer person_3 10);
-    build_act creator deploy_fa2token
+    build_act creator deploy_fa2token;
+    build_act creator deploy_fa2token_client
   ]).
+
+Definition call_client_is_op_act :=
+  let params := Build_is_operator_param 
+      (Build_operator_param zero_address zero_address all_tokens)
+      (Build_callback is_operator_response) in 
+  let msg := other_msg (FA2ClientContract.Call_fa2_is_operator params) in
+  act_call client_contract_addr 0%Z (serialize FA2ClientContract.Msg _ msg).
+
+Definition chain_1 : LocalChain :=
+  unpack_option (my_add_block chain_with_token_deployed 
+  [
+    build_act person_1 call_client_is_op_act
+  ]).
+
+Definition asd := 
+  match (FMap.find client_contract_addr chain_1.(lc_contract_state)) with
+  | Some state => deserialize FA2ClientContract.State _ state
+  | None => None
+  end.
+
+Compute asd.
+
+Definition gClientMsg : G FA2ClientContract.Msg := 
+  let params := Build_is_operator_param 
+    (Build_operator_param zero_address zero_address all_tokens)
+    (Build_callback is_operator_response) in
+  returnGen (other_msg (FA2ClientContract.Call_fa2_is_operator params)).
+Definition gClientAction := liftM (fun msg => 
+  Some (
+    build_act person_1 (
+      act_call token_contract_base_addr 0%Z (serialize FA2ClientContract.Msg _ msg)
+    )
+  )) gClientMsg.
+
+Definition gFA2ChainTraceList max_acts_per_block lc length := 
+  gLocalChainTraceList_fix lc (fun _ _=> 
+    gClientAction) length max_acts_per_block.
+
+Definition token_reachableFrom (lc : LocalChain) pf : Checker := 
+  @reachableFrom AddrSize lc (gFA2ChainTraceList 1) pf.
+
+Definition token_reachableFrom_implies_reachable (lc : LocalChain) pf1 pf2 : Checker := 
+  reachableFrom_implies_reachable lc (gFA2ChainTraceList 1) pf1 pf2.
 
 
 
